proof/modelT.v
@@ -1,0 +1,345 @@
+Require Import Bool Arith List Lia List String Logic.
+Require Import Logic.FunctionalExtensionality.
+Require Import Lists.List.
+Require Import POBF.model.
+Import ListNotations.
+
+Definition ThreadId := nat.
+
+(* The location is bound *)
+(* TODO: add global *)
+Definition Tlocation : Type := prod ThreadId location.
+
+Definition Taccessible: Type := list Tlocation.
+
+Definition eq_Tlocation (i1 i2: Tlocation) : bool := 
+  match i1, i2 with
+  | (tid1, l1), (tid2, l2) => if tid1 =? tid2 then eq_location l1 l2 else false
+  end.
+
+Theorem eq_Tlocation_eq: forall i1 i2, eq_Tlocation i1 i2 = true <-> i1 = i2.
+Proof.
+  split.
+  - destruct i1 eqn:eqi1; destruct i2 eqn:eqi2; unfold eq_Tlocation; 
+    intros; try discriminate H; apply pair_equal_spec; split;
+    destruct (t =? t0) eqn: eqtt0; try apply Nat.eqb_eq; try assumption; try discriminate H. apply eq_location_eq. assumption.
+  - destruct i1 eqn:eqi1; destruct i2 eqn:eqi2; unfold eq_location; 
+    intros; inversion H. unfold eq_Tlocation. rewrite Nat.eqb_refl.
+    apply eq_location_eq. reflexivity.
+Qed.
+
+Lemma eq_Tlocation_refl: forall (l: Tlocation), eq_Tlocation l l = true.
+Proof.
+  intros l. assert (H: l = l). reflexivity.
+  apply eq_Tlocation_eq. reflexivity.
+Qed.
+
+(* ThreadId, as the owner of the cell, is stored in Tcell *)
+Inductive Tcell: Type :=
+  | TAppMem (v: tagged_value) (* note that thread isolation doesn't work on insecure memory! *)
+  | TUnusedMem
+  | TEncMem (t: ThreadId) (z: enc_mem_tag) (v: tagged_value)
+.
+
+Definition Tmemory: Type := Tlocation -> Tcell.
+
+Definition empty_Tmem : Tmemory := 
+  (fun _ => TUnusedMem).
+
+(* This update may not be secure! Compare tid? *)
+Definition Tupdate (s: Tlocation) (v: Tcell) (m: Tmemory) : Tmemory := 
+  match v with
+  | TAppMem _ 
+  | TUnusedMem => fun s' => if (eq_Tlocation s' s) then v else m s'
+  | TEncMem t _ _ => if (fst s =? t) (*Checking if the updating is allowed! *)
+                        then fun s' => if (eq_Tlocation s' s) then v else m s'
+                        else m
+  end.
+
+Definition Taccess (me: Tmemory) (mo: mode) (s: Tlocation) : @result tagged_value := 
+  let c := me s in
+    match mo, c with
+    | _, TUnusedMem => Err([Invalid])
+    | EnclaveMode, TAppMem v => Ok v
+    (* Checking if mem of another thread is accessed *)
+    | EnclaveMode, TEncMem t _ v => if t =? (fst s) then Ok v else Err([NoPriviledge])
+    | NormalMode, TEncMem _ _ _ => Err([NoPriviledge])
+    | NormalMode, TAppMem v => Ok(v)
+    end.
+
+(* We assume that only the enclave memory is thread-specific *)
+Theorem T_access_App_shared: forall (me: Tmemory) tid tid' l v,
+  me (tid, l) = TAppMem v -> me (tid', l) = TAppMem v.
+Proof.
+Admitted.
+
+Theorem T_access_Unused_shared: forall (me: Tmemory) tid tid' l,
+  me (tid, l) = TUnusedMem -> me (tid', l) = TUnusedMem.
+Proof.
+Admitted.
+
+(* secrets find on places other than the zone *)
+Fixpoint Tleaked (me: Tmemory) (vars: Taccessible) : bool := 
+  match vars with
+  | [] => false
+  | l::ls => match me l with
+            (* secrets cannot stay on AppMem or nonzone EncMem *)
+            | TAppMem (_, Secret) => true
+            | TEncMem _ NonzoneMem (_, Secret) => true
+            | _ => Tleaked me ls
+            end
+  end.
+
+Inductive Texp: Type :=
+  | TExpLoc (l: Tlocation)
+  | TExpVal (v: value)
+  | TExpUnary (e: Texp) (op: value -> value)
+  | TExpBinary (e1 e2: Texp) (op: value -> value -> value)
+.
+
+Fixpoint Texp_eval (me: Tmemory) (mo: mode) (e: Texp) : @result value := 
+  match e with
+  | TExpLoc l => match Taccess me mo l with
+                | Ok v => Ok (fst v)
+                | Err e => Err e
+                end
+  | TExpVal v => Ok(v)
+  | TExpUnary e _ => match Texp_eval me mo e with
+                    | Ok _ => Ok(Any)
+                    | e => e
+                    end
+  | TExpBinary e1 e2 _ => let r1 := Texp_eval me mo e1 in
+                         let r2 := Texp_eval me mo e2 in
+                         match r1, r2 with
+                         | Ok _, Ok _ => Ok(Any)
+                         | Err er1, Err er2 => Err(er1 ++ er2)
+                         | Err er1, Ok _ => Err(er1)
+                         | Ok _, Err er2 => Err(er2)
+                         end
+  end.
+
+Definition Texp_as_bool (me: Tmemory) (mo: mode) (e: Texp) : @result bool := 
+  match Texp_eval me mo e with
+  | Ok v => Ok (value_as_bool v)
+  | Err e => Err e
+  end.
+
+
+Fixpoint Texp_prop_tag (me: Tmemory) (mo: mode) (e: Texp) : security_tag := 
+  match e with
+  | TExpLoc l => match Taccess me mo l with
+                | Ok v => (snd v)
+                | Err e => Nonsense
+                end
+  | TExpVal v => Notsecret
+  | TExpUnary e _ => Texp_prop_tag me mo e
+  | TExpBinary e1 e2 _ =>  let t1 := Texp_prop_tag me mo e1 in
+                          let t2 := Texp_prop_tag me mo e2 in
+                          sum_two_tags t1 t2
+  end.
+
+Definition Texp_tagged_val (me: Tmemory) (mo: mode) (e: Texp) : @result tagged_value := 
+  match (Texp_eval me mo e), (Texp_prop_tag me mo e) with
+  | Ok v, t => Ok (v, t)
+  | Err ev, _ => Err ev
+  end.
+
+Inductive Tcom : Type :=
+  | TCNop
+  | TCEenter
+  | TCEexit
+  | TCAsgn (l: Tlocation) (v: Texp)
+  | TCSeq (c1 c2: Tcom)
+  | TCIf (b: Texp) (c1 c2: Tcom)
+  | TCWhile (b: Texp) (c: Tcom)
+  (* Declasification *)
+.
+
+Definition Tstate: Type := Tmemory * mode * Taccessible * errors.
+
+(* Add tid here *)
+Inductive Tcom_eval_critical : ThreadId -> Tcom -> Tstate -> Tstate -> Prop :=
+  | TE_Nop (tid: ThreadId) (me: Tmemory) (mo: mode) (vars: Taccessible) (ers: errors) (ers: errors): 
+    Tcom_eval_critical tid TCNop (me, mo, vars, ers) (me, mo, vars, ers)
+  | TE_Eenter (tid: ThreadId) (me: Tmemory) (mo: mode) (vars: Taccessible) (ers: errors) (Her: ers = []):
+    Tcom_eval_critical tid TCEenter (me, mo, vars, ers) (me, EnclaveMode, vars, ers)
+  | TE_Eexit (tid: ThreadId) (me: Tmemory) (mo: mode) (vars: Taccessible) (ers: errors) (Her: ers = []):
+    Tcom_eval_critical tid TCEexit (me, mo, vars, ers) (me, NormalMode, vars, ers)
+  | TE_Asgn_Ok_enc (tid: ThreadId) (me: Tmemory) (mo: mode) (vars: Taccessible) (ers: errors) (Her: ers = [])
+    (l: Tlocation) (v: Texp) (r: tagged_value) 
+    (Hexp: Texp_tagged_val me mo v = (Ok r)) (Henc: mo = EnclaveMode) 
+    (Ht: (fst l) = tid) (* only assign correct tid! *):
+    (* What if not in the enclave mode? *)
+    (* Write restricted in the Zone! *)
+    Tcom_eval_critical tid (TCAsgn l v) (me, mo, vars, ers) ((Tupdate l (TEncMem tid ZoneMem r) me), mo, (l :: vars), ers)
+  | TE_Asgn_Err_access (tid: ThreadId) (me: Tmemory) (mo: mode) (vars: Taccessible) (ers: errors) (Her: ers = [])
+    (l: Tlocation) (v: Texp) (er: errors) (Hexp: Texp_tagged_val me mo v = (Err er)):
+    Tcom_eval_critical tid (TCAsgn l v) (me, mo, vars, ers) (me, mo, vars, (er ++ ers))
+  | TE_Seq (tid: ThreadId) (st st' st'': Tstate) (c1 c2: Tcom)
+    (Hc1: Tcom_eval_critical tid c1 st st') (Hc2: Tcom_eval_critical tid c2 st' st''):
+    Tcom_eval_critical tid (TCSeq c1 c2) st st''
+  | TE_If_then (tid: ThreadId) (me: Tmemory) (mo: mode) (vars: list Tlocation) (ers: errors) (Her: ers = [])
+    (b: Texp) (c1 c2: Tcom) (st': Tstate):
+    Texp_as_bool me mo b = Ok true -> 
+    Tcom_eval_critical tid c1 (me, mo, vars, ers) st' -> 
+    Tcom_eval_critical tid (TCIf b c1 c2) (me, mo, vars, ers) st'
+  | TE_If_else (tid: ThreadId) (me: Tmemory) (mo: mode) (vars: list Tlocation) (ers: errors) (Her: ers = [])
+    (b: Texp) (c1 c2: Tcom) (st': Tstate):
+    Texp_as_bool me mo b = Ok false -> 
+    Tcom_eval_critical tid c2 (me, mo, vars, ers) st' -> 
+    Tcom_eval_critical tid (TCIf b c1 c2) (me, mo, vars, ers) st'
+  | TE_If_err (tid: ThreadId) (me: Tmemory) (mo: mode) (vars: list Tlocation) (ers: errors) (Her: ers = [])
+    (b: Texp) (c1 c2: Tcom) (st': Tstate) (er: errors):
+    Texp_as_bool me mo b = Err er -> 
+    Tcom_eval_critical tid (TCIf b c1 c2) (me, mo, vars, ers) (me, mo, vars, er ++ ers)
+  | TE_while_true (tid: ThreadId) (me: Tmemory) (mo: mode) (vars: list Tlocation) (ers: errors) (Her: ers = [])
+    (b: Texp) (c: Tcom) (st': Tstate):
+    Texp_as_bool me mo b = Ok true -> 
+    Tcom_eval_critical tid c (me, mo, vars, ers) st' -> 
+    Tcom_eval_critical tid (TCWhile b c) (me, mo, vars, ers) st'
+  | TE_while_false (tid: ThreadId) (me: Tmemory) (mo: mode) (vars: list Tlocation) (ers: errors) (Her: ers = [])
+    (b: Texp) (c: Tcom) (st': state):
+    Texp_as_bool me mo b = Ok false -> 
+    Tcom_eval_critical tid (TCWhile b c) (me, mo, vars, ers) (me, mo, vars, ers)
+  | TE_while_err (tid: ThreadId) (me: Tmemory) (mo: mode) (vars: list Tlocation) (ers: errors) (Her: ers = [])
+    (b: Texp) (c: Tcom) (st': state) (er: errors):
+    Texp_as_bool me mo b = Err er -> 
+    Tcom_eval_critical tid (TCWhile b c) (me, mo, vars, ers) (me, mo, vars, er ++ ers)
+  | TE_Err_ignore (tid: ThreadId) (me: Tmemory) (mo: mode) (vars: Taccessible) (ers: errors) 
+    (Herr: (length ers) >= 1) (c: Tcom):
+    Tcom_eval_critical tid c (me, mo, vars, ers) (me, mo, vars, ers)
+.
+
+(* Singlize the multi-threading state-related data structures *)
+Definition singlize_Tcell (tid: ThreadId) (c: Tcell) := 
+  match c with
+  | TAppMem v => AppMem v
+  | TUnusedMem => UnusedMem
+  | TEncMem t z v
+    => if (t =? tid) then EncMem z v else UnusedMem
+  end.
+
+Fixpoint singlize_Taccessible (tid: ThreadId) (vars: Taccessible) : accessible := 
+  match vars with
+  | [] => []
+  | h :: t => if (fst h =? tid) then (snd h) :: (singlize_Taccessible tid t) else (singlize_Taccessible tid t)
+  end.
+
+Fixpoint singlize_Tmemory (tid: ThreadId) (me: Tmemory) (vars: Taccessible) : memory := 
+  match vars with
+  | [] => empty_mem
+  | h :: t => update (snd h) (singlize_Tcell (fst h) (me h)) (singlize_Tmemory tid me t)
+  end.
+
+Lemma singlize_Tapp_app: forall me tid l v vars,
+  In (tid, l) vars ->
+  me (tid, l) = TAppMem v -> (singlize_Tmemory tid me vars) l = AppMem v.
+Proof.
+  intros. induction vars.
+  - inversion H.
+  - simpl. destruct a. simpl in *. destruct H.
+    + inversion H. subst. unfold singlize_Tcell. rewrite H0. unfold update. rewrite eq_location_refl. reflexivity.
+    + unfold update. destruct (eq_location l l0) eqn:eqll0.
+      * apply eq_location_eq in eqll0. subst.
+        apply T_access_App_shared with (tid':=t) in H0.
+        rewrite H0. simpl. reflexivity.
+      * apply IHvars. assumption.
+Qed.
+
+Lemma singlize_Tunused_unused: forall me tid l vars,
+  In (tid, l) vars ->
+  me (tid, l) = TUnusedMem -> (singlize_Tmemory tid me vars) l = UnusedMem.
+Proof.
+  intros. induction vars.
+  - inversion H.
+  - simpl. destruct a. simpl in *. destruct H.
+    + inversion H. subst. unfold singlize_Tcell. rewrite H0. unfold update. rewrite eq_location_refl. reflexivity.
+    + unfold update. destruct (eq_location l l0) eqn:eqll0.
+      * apply eq_location_eq in eqll0. subst.
+        apply T_access_Unused_shared with (tid':=t) in H0.
+        rewrite H0. simpl. reflexivity.
+      * apply IHvars. assumption.
+Qed.
+
+Definition singlize_Tstate (tid: ThreadId) (st: Tstate) : state := 
+  match st with
+  | (me, mo, vars, ers) => ((singlize_Tmemory tid me vars), mo, (singlize_Taccessible tid vars), ers)
+  end.
+
+Fixpoint singlize_Texp (te: Texp) : exp :=
+  match te with
+  | TExpLoc l => ExpLoc (snd l)
+  | TExpVal v => ExpVal v
+  | TExpUnary e op => ExpUnary (singlize_Texp e) op
+  | TExpBinary e1 e2 op => ExpBinary (singlize_Texp e1) (singlize_Texp e2) op
+  end
+.
+
+Fixpoint singlize_Tcom (tc: Tcom) : com := 
+  match tc with
+  | TCNop => CNop
+  | TCEenter => CEenter
+  | TCEexit => CEexit
+  | TCAsgn l v => CAsgn (snd l) (singlize_Texp v)
+  | TCSeq c1 c2 => CSeq (singlize_Tcom c1) (singlize_Tcom c2)
+  | TCIf b c1 c2 => CIf (singlize_Texp b) (singlize_Tcom c1) (singlize_Tcom c2)
+  | TCWhile b c => CWhile (singlize_Texp b) (singlize_Tcom c)
+  end.
+
+Lemma Texp_eval_singlize_err_prop: forall tid me mo vars v er,
+  Texp_tagged_val me mo v = Err er -> 
+  (exists er', exp_tagged_val (singlize_Tmemory tid me vars) mo (singlize_Texp v) = Err er').
+Proof.
+  intros. induction v; simpl.
+  - destruct l. simpl in *. 
+    unfold Texp_tagged_val in *. unfold Texp_eval in *. unfold Taccess in *.
+    unfold exp_tagged_val. unfold exp_eval. unfold access.
+    destruct mo eqn: mode.
+    + destruct (me (t, l)) eqn: Hl; try inversion H.
+    (* Need a lemma here! *)
+      destruct (singlize_Tmemory tid me vars l) eqn: eql. admit.
+      exists [Invalid]. reflexivity. exists [NoPriviledge]. reflexivity. 
+      destruct (singlize_Tmemory tid me vars l) eqn: eql. admit. exists [Invalid]. reflexivity.
+    exists [NoPriviledge]. reflexivity.
+    + destruct (me (t, l)) eqn:eqt. inversion H.
+      inversion H. assert (Ha: In (tid, l) vars). admit.
+      apply singlize_Tunused_unused with (me:=me) in Ha. rewrite Ha.
+      eauto. apply T_access_Unused_shared with (tid':= tid) in eqt. assumption.
+      destruct (t0 =? t) eqn : eqtt0; simpl in *. 
+      rewrite eqtt0 in H. rewrite eqt in H. inversion H.
+      rewrite eqtt0 in H. admit.
+  - unfold exp_tagged_val. admit.
+  - admit.
+  - admit.
+Admitted.
+
+(* TODO: bool exp transition! *)
+Theorem singlize_exec: forall tid com st st', 
+  Tcom_eval_critical tid com st st' -> com_eval_critical (singlize_Tcom com) (singlize_Tstate tid st) (singlize_Tstate tid st').
+Proof.
+  intros. induction H.
+  (* Nop *)
+  - simpl. apply E_Nop. assumption.
+  (* Eenter *)
+  - simpl. apply E_Eenter. assumption.
+  (* Eexit *)
+  - simpl. apply E_Eexit. assumption.
+  (* Asgn *)
+  - simpl. destruct l. simpl in *. subst. rewrite <- beq_nat_refl with tid in *. rewrite eq_Tlocation_refl.
+    simpl. rewrite <- beq_nat_refl with tid. admit.
+  - apply E_Asgn_Err_access. assumption. 
+  apply Texp_eval_singlize_err_prop in Hexp. admit.
+  (* Seq *)
+  - simpl. apply E_Seq with (st':= (singlize_Tstate tid st')). assumption. assumption.
+  (* If *)
+  - simpl. apply E_If_then. assumption. admit. assumption.
+  - simpl. apply E_If_else. assumption. admit. assumption.
+  - simpl. apply E_If_err. assumption. admit.
+  (* While *)
+  - simpl. apply E_while_true. assumption. admit. assumption.
+  - simpl. apply E_while_false. assumption. admit.
+  - simpl. apply E_while_err. assumption. admit.
+  (* Err_ignore *)
+  - simpl. apply E_Err_ignore. assumption.
+Admitted.
+
